Eff.Template.Equation.Test3.fst
@@ -1,0 +1,88 @@
+module Eff.Template.Equation.Test3
+
+open Eff.Signature
+open Eff.Template
+open Eff.Template.Equation
+open Eff.Template.Equiv
+
+(* Read and write effects for integer state *)
+
+let read = Op "read" #unit #int
+let write = Op "write" #int #unit
+
+let r : sig = singleton read
+let w : sig = singleton write
+let rw : sig = r `union` w
+
+
+(* State equations using templates *)
+
+let st_eq1 a : repr_equation a rw 
+  = { 
+      repr_vctx = [];
+      repr_cctx = [unit];
+      repr_lhs  = (fun vvars cvars -> Node read () (fun y ->
+                                   Node write y (fun y' ->
+                                   repr_cvar cvars 0 y')));
+      repr_rhs  = (fun vvars cvars -> repr_cvar cvars 0 ())
+    }
+
+let st_eq2 a : repr_equation a rw
+  = {
+      repr_vctx = [int];
+      repr_cctx = [int];
+      repr_lhs  = (fun vvars cvars -> Node write (vvar vvars 0) (fun y ->
+                                   Node read () (fun y' ->
+                                   repr_cvar cvars 0 y')));
+      repr_rhs  = (fun vvars cvars -> Node write (vvar vvars 0) (fun y ->
+                                   repr_cvar cvars 0 (vvar vvars 0)))
+    }
+
+let st_eq3 a : repr_equation a rw
+  = {
+      repr_vctx = [int;int];
+      repr_cctx = [unit];
+      repr_lhs  = (fun vvars cvars -> Node write (vvar vvars 0) (fun y ->
+                                   Node write (vvar vvars 1) (fun y' ->
+                                   repr_cvar cvars 0 y')));
+      repr_rhs  = (fun vvars cvars -> Node write (vvar vvars 1) (fun y ->
+                                   repr_cvar cvars 0 y))
+    }
+
+
+
+
+
+
+
+
+
+
+
+
+
+(* ***************************** *)
+
+let st_eq a : repr_equation a rw
+  = {
+      repr_vctx = [int;int;int];
+      repr_cctx = [unit];
+      repr_lhs  = (fun vvars cvars -> Node write (vvar vvars 0) (fun y ->
+                                   Node write (vvar vvars 1) (fun y' ->
+                                   Node write (vvar vvars 2) (fun y'' ->
+                                   repr_cvar cvars 0 y''))));
+      repr_rhs  = (fun vvars cvars -> Node write (vvar vvars 0) (fun y ->
+                                   Node write (vvar vvars 2) (fun y' ->
+                                   repr_cvar cvars 0 y')))
+    }
+
+open FStar.Tactics
+
+let foo a 
+  : Lemma (requires (repr_eq_to_prop (st_eq3 a)))
+          (ensures  (repr_eq_to_prop (st_eq a))) by (norm [delta;zeta;primops;simplify;iota]; dump "foo")
+  = ()
+
+
+
+
